Update syntax of ccsub_infrastructure. Many admitted proofs that no longer work.

CCsub_Infrastructure.v
@@ -4,74 +4,74 @@ Require Import Lia.
 
 Fixpoint fv_ct (T : typ) {struct T} : atoms :=
   match T with
-  | typ_var _ => {}A
-  | C # R => `cse_fvars` C `u`A fv_ct R
-  | ⊤ => {}A
-  | ∀ (S') T => fv_ct S' `u`A fv_ct T
-  | ∀ [R] T => fv_ct R `u`A fv_ct T
+  | typ_var _ => {}a
+  | C # R => `cse_fvars` C `union`a fv_ct R
+  | ⊤ => {}a
+  | ∀ (S') T => fv_ct S' `union`a fv_ct T
+  | ∀ [R] T => fv_ct R `union`a fv_ct T
   | □ T => fv_ct T
   end.
 
 Fixpoint fv_tt (T : typ) {struct T} : atoms :=
   match T with
-  | var_b J => {}A
+  | var_b J => {}a
   | var_f X => singleton X
   | C # R => fv_tt R
-  | ⊤ => {}A
-  | ∀ (S') T => fv_tt S' `u`A fv_tt T
-  | ∀ [R] T => fv_tt R `u`A fv_tt T
+  | ⊤ => {}a
+  | ∀ (S') T => fv_tt S' `union`a fv_tt T
+  | ∀ [R] T => fv_tt R `union`a fv_tt T
   | □ T => fv_tt T
   end.
 
 Fixpoint fv_ce (e : exp) {struct e} : atoms :=
   match e with
-  | exp_var_like _ => {}A
-  | λ (V) e1 => fv_ct V `u`A fv_ce e1
-  | _ @ _ => {}A
-  | let= e in C => fv_ce e `u`A fv_ce C
-  | Λ [V] e1 => fv_ct V `u`A fv_ce e1
+  | exp_var_like _ => {}a
+  | λ (V) e1 => fv_ct V `union`a fv_ce e1
+  | _ @ _ => {}a
+  | let= e in C => fv_ce e `union`a fv_ce C
+  | Λ [V] e1 => fv_ct V `union`a fv_ce e1
   | _ @ [V] => fv_ct V
-  | box _ => {}A
+  | box _ => {}a
   | C ⟜ x => `cse_fvars` C
   end.
 
 Fixpoint fv_te (e : exp) {struct e} : atoms :=
   match e with
-  | exp_var_like _ => {}A
-  | λ (V) e1  => fv_tt V `u`A fv_te e1
-  | _ @ _ => {}A
-  | let= e in C => fv_te e `u`A fv_te C
-  | Λ [V] e1 => fv_tt V `u`A fv_te e1
+  | exp_var_like _ => {}a
+  | λ (V) e1  => fv_tt V `union`a fv_te e1
+  | _ @ _ => {}a
+  | let= e in C => fv_te e `union`a fv_te C
+  | Λ [V] e1 => fv_tt V `union`a fv_te e1
   | _ @ [V] => fv_tt V
-  | box _ => {}A
-  | C ⟜ x => {}A
+  | box _ => {}a
+  | C ⟜ x => {}a
   end.
 
 Definition fv_vv (v : var_like) : atoms :=
   match v with
   | var_like_var (var_f x) => singleton x
-  | var_like_var (var_b _) => {}A
-  | var_like_loc _ => {}A
+  | var_like_var (var_b _) => {}a
+  | var_like_loc _ => {}a
   end.
 
 Fixpoint fv_ve (e : exp) {struct e} : atoms :=
   match e with
   | var_like_var v => fv_vv v
-  | var_like_loc l => {}A
+  | var_like_loc l => {}a
   | λ (V) e1 => fv_ve e1
-  | x @ y => fv_vv x `u`A fv_vv y
-  | let= e in C => fv_ve e `u`A fv_ve C
+  | x @ y => fv_vv x `union`a fv_vv y
+  | let= e in C => fv_ve e `union`a fv_ve C
   | Λ [V] e1 => fv_ve e1
   | x @ [V] => fv_vv x
   | box x => fv_vv x
-  | C ⟜ x => `cse_fvars` C `u`A fv_vv x
+  | C ⟜ x => `cse_fvars` C `union`a fv_vv x
   end.
 
 Fixpoint fv_cctx (E : ctx) {struct E} : atoms :=
   match E with
-  | nil => {}A
-  | (_, bind_typ T) :: F => fv_ct T `u`A fv_cctx F
-  | (_, bind_sub T) :: F => fv_ct T `u`A fv_cctx F
+  | nil => {}a
+  | (_, bind_typ T) :: F => fv_ct T `union`a fv_cctx F
+  | (_, bind_sub T) :: F => fv_ct T `union`a fv_cctx F
   end.
 
 Fixpoint subst_tt (Z : atom) (U : typ) (T : typ) {struct T} : typ :=
@@ -151,7 +151,7 @@ Ltac gather_atoms :=
   let H := gather_atoms_with (fun x : typ => fv_ct x) in
   let I := gather_atoms_with (fun x : exp => fv_ce x) in
   let J := gather_atoms_with (fun x : ctx => fv_cctx x) in
-  constr:(A `u`A B `u`A C `u`A D `u`A E `u`A F `u`A G `u`A H `u`A I `u`A J).
+  constr:(A `union`a B `union`a C `union`a D `union`a E `union`a F `union`a G `union`a H `union`a I `union`a J).
 
 Tactic Notation "pick" "fresh" ident(x) :=
   let L := gather_atoms in (pick fresh x for L).
@@ -234,19 +234,21 @@ Lemma varN_weakening : forall n m v,
   varN n v ->
   n <= m ->
   varN m v.
-Proof with eauto*.
+Admitted.
+(* Proof with eauto*.
   intros.
   induction H; constructor; lia.
-Qed.
+Qed. *)
 
 Lemma csetN_weakening : forall n m C,
   csetN n C ->
   n <= m ->
   csetN m C.
-Proof with eauto*.
+Admitted.
+(* Proof with eauto*.
   intros.
   induction H; constructor... lia.
-Qed.
+Qed. *)
 
 Lemma typeN_weakening : forall n m T,
   typeN n T ->
@@ -273,7 +275,8 @@ Qed.
 Lemma open_vt_typeN_aux : forall n S v,
   typeN n (open_vt n S v) ->
   typeN (`succ` n) v.
-Proof with eauto*.
+Admitted.
+(* Proof with eauto*.
   intros.
   destruct v...
   unfold open_vt in H.
@@ -281,7 +284,7 @@ Proof with eauto*.
   inversion H; inversion H0; inversion H5; subst...
   apply typeN_pure, typeN_var, varN_b.
   lia.
-Qed.
+Qed. *)
 
 Lemma open_tt_rec_typeN_aux : forall n S T,
   typeN n (open_tt_rec n S T) ->
@@ -303,8 +306,7 @@ Proof with eauto using open_vt_typeN_aux.
 { clear open_tt_rec_pure_typeN_aux.
   intros * H.
   dependent induction H.
-  - Case "bound variable".
-    unfold open_tt_rec in x.
+  - unfold open_tt_rec in x.
     destruct R; simpl in x.
     1: {
       destruct v0...
@@ -316,8 +318,7 @@ Proof with eauto using open_vt_typeN_aux.
       lia.
     }
     all: discriminate x.
-  - Case "⊤".
-    destruct R; simpl in x...
+  - destruct R; simpl in x...
     1: {
       destruct v...
       simpl in x.
@@ -325,8 +326,7 @@ Proof with eauto using open_vt_typeN_aux.
       inversion x.
     }
     all: discriminate x.
-  - Case "∀ (S') T".
-    destruct R; simpl in x...
+  - destruct R; simpl in x...
     1: {
       destruct v...  
       simpl in x.
@@ -336,8 +336,7 @@ Proof with eauto using open_vt_typeN_aux.
     injection x as x; subst.
     apply typeN_arr...
     all: discriminate x.
-  - Case "∀ [R] T". 
-    destruct R; simpl in x...
+  - destruct R; simpl in x...
     1: {
       destruct v...
       simpl in x.
@@ -347,13 +346,12 @@ Proof with eauto using open_vt_typeN_aux.
     2: {
       injection x as x1 x2.
       apply typeN_all...
-      eapply open_tt_rec_typeN_aux with (S0 := S).
+      eapply open_tt_rec_typeN_aux with (S := S).
       rewrite <- x2.
       apply H0.
     }
     all: discriminate x.
-  - Case "□ T".
-    destruct R; simpl in x...
+  - destruct R; simpl in x...
     1: {
       unfold open_vt in x.
       destruct v...  
@@ -374,7 +372,8 @@ Lemma open_ct_rec_typeN_aux : forall n S T,
 with open_ct_rec_pure_typeN_aux : forall n S R,
   pure_typeN n (open_ct_rec n S R) ->
   pure_typeN (`succ` n) R.
-Proof with eauto*.
+Admitted.
+(* Proof with eauto*.
 { clear open_ct_rec_typeN_aux.
   intros * H.
   dependent induction H...
@@ -404,13 +403,14 @@ Proof with eauto*.
   1: destruct v; destruct v0; inversion H; injection x as x; subst...
   all: injection x; intros; subst...
 }
-Qed.
+Qed. *)
 
 Lemma type_to_type0 : forall T,
   type T -> typeN 0 T
 with pure_type_to_pure_type0 : forall R,
   pure_type R -> pure_typeN 0 R.
-Proof with eauto.
+Admitted.
+(* Proof with eauto.
 { clear type_to_type0.
   intros * H.
   dependent induction H...
@@ -434,7 +434,7 @@ Proof with eauto.
     unfold open_ct in H0.
     eapply (open_tt_rec_typeN_aux 0 X)...
 }
-Qed.
+Qed. *)
 
 Hint Extern 1 (_ >= _) => lia : core.
 
@@ -442,14 +442,15 @@ Lemma open_vt_typeN : forall n m S v,
   varN n v ->
   m >= n ->
   typ_var v = open_vt m S v.
-Proof with eauto*.
+Admitted.
+(* Proof with eauto*.
   intros.
   unfold open_vt.
   destruct v...
   destruct (m === n0); subst...
   inversion H.
   lia.
-Qed.
+Qed. *)
 
 Lemma open_tt_rec_typeN : forall n m S T,
   typeN n T ->
@@ -467,14 +468,12 @@ Lemma open_tt_rec_type : forall T U k,
   T = open_tt_rec k U T.
 Proof with auto*.
   intros * [R | C R].
-  - Case "R".
-    apply open_tt_rec_typeN with (n := k)...
+  - apply open_tt_rec_typeN with (n := k)...
     apply typeN_pure.
     apply pure_type_to_pure_type0 in H.
     apply pure_typeN_weakening with (m := k) in H...
     lia.
-  - Case "C # R".
-    simpl.
+  - simpl.
     f_equal...
     apply open_tt_rec_typeN with (n := k)...
     apply typeN_pure.
@@ -487,23 +486,24 @@ Qed.
     identity. *)
 
 Lemma subst_tt_fresh : forall Z U T,
-  Z ∉ (fv_tt T `u`A fv_ct T) ->
+  Z ∉ (fv_tt T `union`a fv_ct T) ->
   T = subst_tt Z U T.
-Proof with auto*.
+Admitted.
+(* Proof with auto*.
   intros Z U T.
   induction T; simpl; intro H; f_equal...
-  - Case "variable".
-    destruct v...
+  - destruct v...
     destruct (a == Z)...
     contradict H.
     fsetdec.
-Qed.
+Qed. *)
 
 Lemma subst_tt_open_tt_rec : forall T1 T2 X P k,
   type P ->
   subst_tt X P (open_tt_rec k T2 T1) =
   open_tt_rec k (subst_tt X P T2) (subst_tt X P T1).
-Proof with auto*.
+Admitted.
+(* Proof with auto*.
   intros.
   generalize dependent k.
   induction T1; intros k; simpl; f_equal...
@@ -513,7 +513,7 @@ Proof with auto*.
     apply open_tt_rec_type, H.
   - Case "n".
     destruct (k === n); subst...
-Qed.
+Qed. *)
 
 (** The next lemma is a direct corollary of the immediately preceding
     lemma---the index is specialized to zero. *)
@@ -536,13 +536,14 @@ Lemma subst_tt_open_tt_var : forall (X Y:atom) P T,
   Y <> X ->
   type P ->
   open_tt (subst_tt X P T) Y = subst_tt X P (open_tt T Y).
-Proof with auto*.
+Admitted.
+(* Proof with auto*.
   intros X Y P T Neq Wu.
   unfold open_tt.
   rewrite subst_tt_open_tt_rec...
   simpl.
   destruct (Y == X)...
-Qed.
+Qed. *)
 
 (** The next lemma states that opening a term is equivalent to first
     opening the term with a fresh name and then substituting for the
@@ -550,9 +551,10 @@ Qed.
     the version we use in practice. *)
 
 Lemma subst_tt_intro_rec : forall X T2 U k,
-  X ∉ (fv_tt T2 `u`A fv_ct T2) ->
+  X ∉ (fv_tt T2 `union`a fv_ct T2) ->
   open_tt_rec k U T2 = subst_tt X U (open_tt_rec k X T2).
-Proof with auto*.
+Admitted.
+(* Proof with auto*.
   induction T2; intros U k Fr; simpl in *; f_equal...
   - Case "variable".
     unfold open_vt.
@@ -565,13 +567,13 @@ Proof with auto*.
       destruct (k === n); subst...
       simpl.
       destruct (X == X); try (contradict n; reflexivity)...
-Qed.
+Qed. *)
 
 (** The next lemma is a direct corollary of the immediately preceding
     lemma---the index is specialized to zero.  *)
 
 Lemma subst_tt_intro : forall X T2 U,
-  X ∉ (fv_tt T2 `u`A fv_ct T2) ->
+  X ∉ (fv_tt T2 `union`a fv_ct T2) ->
   open_tt T2 U = subst_tt X U (open_tt T2 X).
 Proof with auto*.
   intros.
@@ -627,7 +629,7 @@ Hint Resolve csetN_weakening varN_weakening typeN_weakening : core.
 Lemma open_cset_csetN : forall n C D,
   csetN n C ->
   C = open_cse n D C.
-Proof with eauto*.
+Proof.
   intros.
   unfold open_cse.
   induction C; auto; inversion H; simpl in *.
@@ -637,7 +639,7 @@ Qed.
 
 Lemma cse_join_in :
   forall X C1 C2, X ∉ `cse_fvars` (cse_join C1 C2) -> X ∉ `cse_fvars` C1 /\ X ∉ `cse_fvars` C2.
-Proof with eauto*.
+Proof.
   intros; split; unfold not; intros; unfold not in H; apply H; simpl;
   apply AtomSetFacts.union_iff; auto.
 Qed.
@@ -645,7 +647,7 @@ Qed.
 Lemma subst_cse_intro : forall X k D C,
   X ∉ `cse_fvars` C ->
   open_cse k D C = subst_cse X D (open_cse k (cse_fvar X) C).
- Proof with eauto*.
+ Proof.
   intros.
   unfold open_cse.
   (* destruct_set_mem k C. *)
@@ -670,7 +672,7 @@ Lemma subst_te_open_te_rec : forall e T X U k,
   pure_type U ->
   subst_te X U (open_te_rec k T e) =
     open_te_rec k (subst_tt X U T) (subst_te X U e).
-Proof with eauto*.
+Proof.
   intros.
   generalize dependent k.
   induction e; intros k; simpl; f_equal; auto using subst_tt_open_tt_rec.
@@ -680,24 +682,26 @@ Lemma subst_te_open_te_var : forall (X Y:atom) U e,
   Y <> X ->
   pure_type U ->
   open_te (subst_te X U e) Y = subst_te X U (open_te e Y).
-Proof with auto*.
+Admitted.
+(* Proof with auto*.
   intros X Y U e Neq WU.
   unfold open_te.
   rewrite subst_te_open_te_rec...
   simpl.
   destruct (Y == X)...
-Qed.
+Qed. *)
 
 Lemma subst_te_intro_rec : forall X e U k,
-  X ∉ (fv_te e `u`A fv_ce e) ->
+  X ∉ (fv_te e `union`a fv_ce e) ->
   open_te_rec k U e = subst_te X U (open_te_rec k X e).
-Proof.
+Admitted.
+(* Proof.
   induction e; intros U k Fr; simpl in *; f_equal;
     auto using subst_cse_intro, subst_tt_intro_rec.
-Qed.
+Qed. *)
 
 Lemma subst_te_intro : forall X e U,
-  X ∉ (fv_te e `u`A fv_ce e) ->
+  X ∉ (fv_te e `union`a fv_ce e) ->
   open_te e U = subst_te X U (open_te e X).
 Proof with auto*.
   intros.
@@ -718,7 +722,8 @@ Qed.
 Lemma open_ct_rec_type : forall T C k,
   type T ->
   T = open_ct_rec k C T.
-Proof with auto using type_to_type0.
+Admitted.
+(* Proof with auto using type_to_type0.
   intros.
   generalize dependent k.
   induction T; intros k; simpl; f_equal; inversion H; inversion H0; subst...
@@ -731,7 +736,7 @@ Proof with auto using type_to_type0.
     apply open_tt_rec_typeN_aux with (S0 := X)...
   - induction H2; auto.
     -- simpl. f_equal; try apply IHcset1; try apply IHcset2; auto. 
-Qed.
+Qed. *)
 
 (*
    TODO maybe we need to strengthen the lemma again for other use cases?
@@ -765,9 +770,9 @@ Qed.
 (** This section follows the structure of the previous two sections. *)
 
 Lemma subst_cse_fresh : forall x C1 C2,
-  x `notin` (cse_fvars C1) ->
+  x `notin`a (cse_fvars C1) ->
   C1 = subst_cse x C2 C1.
-Proof with eauto.
+Proof.
   intros. induction C1; auto.
   - simpl. destruct (x == a).
     -- subst. exfalso. unfold not in H. apply H. simpl. fsetdec.
@@ -788,20 +793,22 @@ Qed.
 Lemma subst_vv_fresh : forall (x : atom) u v,
   x ∉ fv_vv v ->
   v = subst_vv x u v.
-Proof with eauto*.
+Admitted.
+(* Proof with eauto*.
   intros.
   unfold fv_vv, subst_vv in *.
   destruct v... destruct v...
   destruct (a == x); subst...
   fsetdec.
-Qed.
+Qed. *)
 
 Lemma subst_ve_fresh : forall (x : atom) u c e,
-  x ∉ (fv_ve e `u`A fv_ce e) ->
+  x ∉ (fv_ve e `union`a fv_ce e) ->
   e = subst_ve x u c e.
-Proof with auto using subst_vv_fresh, subst_ct_fresh, subst_cse_fresh.
+Admitted.
+(* Proof with auto using subst_vv_fresh, subst_ct_fresh, subst_cse_fresh.
   induction e;  intros; simpl in *; f_equal... destruct v... destruct v... notin_simpl. destruct (a == x)... fsetdec.
-Qed.
+Qed. *)
 
 Lemma subst_ct_open_rec : forall t x k c1 c2,
   cset c1 ->
@@ -822,10 +829,8 @@ Lemma subst_ct_intro_rec : forall X T2 C k,
   open_ct_rec k C T2 = subst_ct X C (open_ct_rec k (cse_fvar X) T2).
 Proof with auto*.
   induction T2; intros C k Fr; simpl in *; f_equal...
-  - Case "v".
-    destruct v...
-  - Case "c # T2".
-    apply subst_cc_intro_rec.
+  - destruct v...
+  - apply subst_cc_intro_rec.
     fsetdec.
 Qed.
 
@@ -895,16 +900,17 @@ Lemma subst_ct_open_ct_var : forall (x y : atom) c t,
   y <> x ->
   cset c ->
   open_ct (subst_ct x c t) (cse_fvar y) = subst_ct x c (open_ct t (cse_fvar y)).
-Proof with auto*.
+Admitted.
+  (* Proof with auto*.
   intros *; intros Neq Wu.
   unfold open_ct.
   symmetry.
   apply subst_ct_open_ct_rec...
-Qed.
+Qed. *)
 
 Lemma subst_te_open_ve_rec : forall e z c Z P k,
   type P ->
-  Z ∉ (`cse_fvars` c `u`A {z}A) ->
+  Z `notin`a (`cse_fvars` c `union`a {{z}}a) ->
   subst_te Z P (open_ve_rec k z c e) =
     open_ve_rec k z c (subst_te Z P e).
 Proof with eauto using subst_tt_open_ct_rec, subst_cset_open_cset_fresh.
@@ -913,7 +919,7 @@ Qed.
 
 Lemma subst_te_open_ve : forall e z c Z P,
   type P ->
-  Z ∉ (`cse_fvars` c `u`A {z}A) ->
+  Z ∉ (`cse_fvars` c `union`a {{z}}a) ->
   subst_te Z P (open_ve e z c) = open_ve (subst_te Z P e) z c.
 Proof with auto*.
   intros.
@@ -923,7 +929,7 @@ Qed.
 
 Lemma subst_te_open_ve_var : forall Z (x : atom) P e c,
   type P ->
-  Z ∉ (`cse_fvars` c `u`A {x}A) ->
+  Z ∉ (`cse_fvars` c `union`a {{x}}a) ->
   open_ve (subst_te Z P e) x c = subst_te Z P (open_ve e x c).
 Proof with auto*.
   intros.
@@ -932,19 +938,20 @@ Qed.
 
 Lemma subst_ct_open_vt_fresh : forall z c k P v,
   cset c ->
-  z ∉ (fv_ct P `u`A fv_tt P) ->
+  z ∉ (fv_ct P `union`a fv_tt P) ->
   subst_ct z c (open_vt k P v) = open_tt_rec k P v.
-Proof with eauto.
+Admitted.
+(* Proof with eauto.
   intros * Capt NotIn.
   induction P; unfold open_vt; destruct v; simpl in *...
   all: destruct (k === n); subst; simpl; f_equal...
   - destruct v0...
   - symmetry. apply subst_cse_fresh...
-Qed.
+Qed. *)
 
 Lemma subst_ct_open_tt_rec_fresh : forall c z P t k,
   cset c ->
-  z ∉ (fv_ct P `u`A fv_tt P) ->
+  z ∉ (fv_ct P `union`a fv_tt P) ->
   subst_ct z c (open_tt_rec k P t) = open_tt_rec k P (subst_ct z c t).
 Proof with eauto using subst_ct_open_vt_fresh.
   induction t; intros; simpl; f_equal...
@@ -953,7 +960,7 @@ Qed.
 
 Lemma subst_ve_open_te_rec_fresh : forall e P z u c k,
   cset c ->
-  z ∉ (fv_ct P `u`A fv_tt P) ->
+  z ∉ (fv_ct P `union`a fv_tt P) ->
   subst_ve z u c (open_te_rec k P e) = open_te_rec k P (subst_ve z u c e).
 Proof with eauto using subst_cset_open_cset_fresh, subst_ct_open_tt_rec_fresh.
   induction e; intros * Hc Hfv; simpl; f_equal... 
@@ -962,7 +969,7 @@ Qed.
 
 Lemma subst_ve_open_te_fresh : forall e P z u c,
   cset c ->
-  z ∉ (fv_ct P `u`A fv_tt P) ->
+  z ∉ (fv_ct P `union`a fv_tt P) ->
   subst_ve z u c (open_te e P) = open_te (subst_ve z u c e) P.
 Proof with auto*.
   intros.
@@ -974,10 +981,11 @@ Lemma subst_ve_open_te_var : forall z (X : atom) u c e,
   z <> X ->
   cset c ->
   open_te (subst_ve z u c e) X = subst_ve z u c (open_te e X).
-Proof with auto*.
+Admitted.
+(* Proof with auto*.
   intros.
   rewrite subst_ve_open_te_fresh...
-Qed.
+Qed. *)
 
 (* if x is fresh, opening with {x} and then substituting is the same as opening directly. *)
 Lemma open_ct_subst_ct_var : forall x c t k,
@@ -993,16 +1001,18 @@ Lemma subst_ct_open_tt_var : forall (X Y:atom) C T,
   Y <> X ->
   cset C ->
   open_tt (subst_ct X C T) Y = subst_ct X C (open_tt T Y).
-Proof with auto*.
+Admitted.
+(* Proof with auto*.
   intros X Y P T Neq Wu.
   unfold open_tt.
   rewrite subst_ct_open_tt_rec_fresh...
-Qed.
+Qed. *)
 
 Lemma subst_vv_intro : forall k x u v,
   x ∉ fv_vv v ->
   open_vv k u v = subst_vv x u (open_vv k x v).
-Proof with eauto*.
+Admitted.
+(* Proof with eauto*.
   intros.
   unfold open_vv, fv_vv, subst_vv in *.
   destruct v. destruct v.
@@ -1011,13 +1021,14 @@ Proof with eauto*.
   * destruct (k === n); subst...
     destruct (x == x)...
   * reflexivity. 
-Qed.
+Qed. *)
 
 Lemma subst_vv_open_vv : forall x u k y v,
   y <> x ->
   fvar_like u ->
   subst_vv x u (open_vv k y v) = open_vv k y (subst_vv x u v).
-Proof with eauto*.
+Admitted.
+(* Proof with eauto*.
   intros * Neq Fvar.
   destruct v. destruct v; simpl. 
   - destruct (a == x); simpl; subst...
@@ -1025,22 +1036,23 @@ Proof with eauto*.
   - destruct (k === n); simpl...
     destruct (y == x); simpl; subst...
   - reflexivity.
-Qed.
+Qed. *)
 
 Lemma subst_ve_intro_rec : forall x e u c k,
-  x ∉ (fv_ve e `u`A fv_ce e) ->
+  x ∉ (fv_ve e `union`a fv_ce e) ->
   open_ve_rec k u c e = subst_ve x u c (open_ve_rec k x (cse_fvar x) e).
-Proof with eauto using open_ct_subst_ct_var, subst_vv_intro, subst_cse_intro.
+Admitted.
+  (* Proof with eauto using open_ct_subst_ct_var, subst_vv_intro, subst_cse_intro.
   induction e; intros u c' k Fr; simpl in *; f_equal... destruct v... destruct v...
   - notin_simpl. simpl. destruct (a == x). rewrite e in H1. 
   contradiction. reflexivity.
   - notin_simpl. simpl. destruct (k === n). destruct (x == x). reflexivity. contradiction.
     reflexivity.
-Qed.
+Qed. *)
 
 
 Lemma subst_ve_intro : forall x e u c,
-  x ∉ (fv_ve e `u`A fv_ce e) ->
+  x ∉ (fv_ve e `union`a fv_ce e) ->
   open_ve e u c = subst_ve x u c (open_ve e x (cse_fvar x)).
 Proof with auto*.
   intros.
@@ -1054,7 +1066,8 @@ Lemma subst_ve_open_ve_rec : forall e x y u c1 c2 k,
   cset c1 ->
   subst_ve x u c1 (open_ve_rec k y c2 e) =
     open_ve_rec k y (subst_cse x c1 c2) (subst_ve x u c1 e).
-Proof with auto using subst_vv_open_vv, subst_ct_open_rec, subst_cset_open_cset_fresh.
+Admitted.
+    (* Proof with auto using subst_vv_open_vv, subst_ct_open_rec, subst_cset_open_cset_fresh.
   intros * Neq Fvar Capt.
   revert k.
   induction e; intros k; simpl; f_equal... destruct v. destruct v...
@@ -1062,7 +1075,7 @@ Proof with auto using subst_vv_open_vv, subst_ct_open_rec, subst_cset_open_cset_
   - simpl. destruct (k === n); subst... destruct (y == x); subst... fsetdec.
   - simpl. f_equal; apply subst_cset_open_cset_fresh; auto.
   - destruct u; simpl in *; inversion Fvar; subst...
-Qed.
+Qed. *)
 
 Lemma subst_ve_open_ve_var : forall (x y : atom) u c e,
   y <> x ->
@@ -1070,13 +1083,14 @@ Lemma subst_ve_open_ve_var : forall (x y : atom) u c e,
   cset c ->
   open_ve (subst_ve x u c e) y (cse_fvar y) =
   subst_ve x u c (open_ve e y (cse_fvar y)).
-Proof with auto*.
+Admitted.
+(* Proof with auto*.
   intros x y u c e Neq Fvar Wc.
   unfold open_ve.
   rewrite subst_ve_open_ve_rec...
   simpl.
   destruct (x == y)...
-Qed.
+Qed. *)
 
 (* *********************************************************************** *)
 (** * #<a name="lc"></a># Local closure is preserved under substitution *)
@@ -1094,7 +1108,8 @@ with subst_tt_pure_type : forall Z P T,
   pure_type T ->
   pure_type P ->
   pure_type (subst_tt Z P T).
-Proof with auto.
+Admitted.
+(* Proof with auto.
 { clear subst_tt_type.
   intros Z P T HT HP.
   induction HT; simpl...
@@ -1102,27 +1117,25 @@ Proof with auto.
 { clear subst_tt_pure_type.
   intros Z P T HT HP.
   induction HT; simpl...
-  - Case "X".
-    destruct (X == Z); subst...
-  - Case "∀ (S') T".
-    pick fresh Y and apply type_arr...
+  - destruct (X == Z); subst...
+  - pick fresh Y and apply type_arr...
     rewrite <- subst_tt_open_ct...
-  - Case "∀ [R] T".
-    pick fresh Y and apply type_all...
+  - pick fresh Y and apply type_all...
     rewrite subst_tt_open_tt_var...
 }
-Qed.
+Qed. *)
 
-Local Hint Extern 1 (~ AtomSet.F.In _ _) => simpl_env in *; [fsetdec] : core.
+Local Hint Extern 1 (~ AtomSetImpl.In _ _) => simpl_env in *; [fsetdec] : core.
 
 Lemma subst_ct_open_fresh : forall k z C T X,
   (* X fresh requirement here in z c T *)
-  X ∉ (singleton z `u`A fv_tt T `u`A fv_ct T)
+  X ∉ (singleton z `union`a fv_tt T `union`a fv_ct T)
     /\ X ∉ `cse_fvars` C ->
   cset C ->
   (open_ct_rec k (cse_fvar X) (subst_ct z C T)) =
     (subst_ct z C (open_ct_rec k (cse_fvar X) T)).
-Proof with eauto.
+Admitted.
+(* Proof with eauto.
   intros k z C T X HXfresh HCfresh.
   revert k.
   induction T; intro k; simpl in *; try reflexivity; try destruct v; f_equal...
@@ -1131,7 +1144,7 @@ Proof with eauto.
   - exact HCfresh.
   - constructor.
   - destruct HXfresh. notin_simpl. simpl. fsetdec.
-Qed.
+Qed. *)
 
 Lemma subst_cse_cset: forall X C D,
   cset C ->
@@ -1152,7 +1165,8 @@ with subst_ct_pure_type : forall R z c,
   pure_type R ->
   cset c ->
   pure_type (subst_ct z c R).
- Proof with auto*.
+Admitted.
+ (* Proof with auto*.
 { clear subst_ct_type.
   intros * Typ ?.
   induction Typ; simpl...
@@ -1183,7 +1197,7 @@ with subst_ct_pure_type : forall R z c,
     }
     rewrite H0...
 }
-Qed.
+Qed. *)
 
 (* *********************************************************************** *)
 (** * #<a name="auto"></a># Automation *)
@@ -1239,7 +1253,8 @@ Lemma open_ct_subst_tt : forall x C S T,
   type S ->
   x ∉ `cse_fvars` C ->
   open_ct (subst_tt x S T) C = subst_tt x S (open_ct T C).
-Proof with auto
+Admitted.
+(* Proof with auto
     using open_cse_cset,
           open_ct_rec_type,
           subst_ct_open_rec,
@@ -1252,16 +1267,17 @@ Proof with auto
   erewrite subst_tt_open_ct_rec.
   erewrite <-subst_ct_intro_rec.
   all: eauto.
-Qed.
+Qed. *)
 
 Lemma subst_tt_open_ct_var : forall (X y:atom) P T,
   y <> X ->
   type P ->
   open_ct (subst_tt X P T) (cse_fvar y) = subst_tt X P (open_ct T (cse_fvar y)).
-Proof with auto*.
+Admitted.
+  (* Proof with auto*.
   intros *; intros Neq Wu.
   unfold open_ct.
   symmetry.
   apply subst_tt_open_ct_rec; trivial.
   notin_solve.
-Qed.
+Qed. *)
